tactics: unthunk everything

ulib/FStar.Tactics.Builtins.fst
@@ -9,64 +9,64 @@ open FStar.Reflection.Types
 open FStar.Tactics.Types
 
 assume private val __embed  : a:Type -> a -> __tac term
-unfold let quote #a (x:a) : tactic term = fun () -> TAC?.reflect (__embed a x)
+unfold let quote #a (x:a) : Tac term = TAC?.reflect (__embed a x)
 
 assume private val __fail : a:Type -> string -> __tac a
-let fail (#a:Type) (msg:string) : tactic a = fun () -> TAC?.reflect (__fail a msg)
+let fail (#a:Type) (msg:string) : Tac a = TAC?.reflect (__fail a msg)
 
 assume private val __top_env     : __tac env
 (** [top_env] returns the environment where the tactic started running.
  * This works even if no goals are present. *)
-let top_env = fun () -> TAC?.reflect __top_env
+let top_env () = TAC?.reflect __top_env
 
 assume private val __cur_env     : __tac env
 (** [cur_env] returns the current goal's environment *)
-let cur_env = fun () -> TAC?.reflect __cur_env
+let cur_env () = TAC?.reflect __cur_env
 
 assume private val __cur_goal    : __tac term
 (** [cur_goal] returns the current goal's type *)
-let cur_goal = fun () -> TAC?.reflect __cur_goal
+let cur_goal () = TAC?.reflect __cur_goal
 
 assume private val __cur_witness : __tac term
 (** [cur_witness] returns the current goal's witness *)
-let cur_witness = fun () -> TAC?.reflect __cur_witness
+let cur_witness () = TAC?.reflect __cur_witness
 
 assume private val __is_guard   : __tac bool
 (** [is_guard] returns whether the current goal arised from a typechecking guard *)
-let is_guard = fun () -> TAC?.reflect __is_guard
+let is_guard () = TAC?.reflect __is_guard
 
 assume private val __refine_intro : __tac unit
 (** [refine_intro] will turn a goal of shape [w : x:t{phi}]
 into [w : t] and [phi{w/x}] *)
-let refine_intro = fun () -> TAC?.reflect __refine_intro
+let refine_intro () = TAC?.reflect __refine_intro
 
 assume private val __tc : term -> __tac term
 (** [tc] returns the type of a term in the current environment,
 or fails if it is untypeable. *)
-let tc (t : term) = fun () -> TAC?.reflect (__tc t)
+let tc (t : term) = TAC?.reflect (__tc t)
 
 assume private val __unshelve : term -> __tac unit
 (** [tc] returns the type of a term in the current environment,
 or fails if it is untypeable. *)
-let unshelve (t : term) = fun () -> TAC?.reflect (__unshelve t)
+let unshelve (t : term) = TAC?.reflect (__unshelve t)
 
 assume private val __unquote : #a:Type -> term -> __tac a
 (** [unquote t] with turn a quoted term [t] into an actual value, of
 any type. This will fail at tactic runtime if the quoted term does not
 typecheck to type [a]. *)
-let unquote (#a:Type) (t:term) : tactic a = fun () -> TAC?.reflect (__unquote #a t)
+let unquote (#a:Type) (t:term) : Tac a = TAC?.reflect (__unquote #a t)
 
 assume private val __trytac : #a:Type -> __tac a -> __tac (option a)
 (** [trytac t] will attempt to run [t] and allow to recover from a failure.
 If [t] succeeds with return value [a], [trytac t] returns [Some a].
 On failure, it returns [None]. See also [or_else].
 *)
-let trytac (t : tactic 'a) = fun () -> TAC?.reflect (__trytac (reify_tactic t))
+let trytac (t : unit -> Tac 'a) = TAC?.reflect (__trytac (reify (t ())))
 
 assume private val __trivial  : __tac unit
 (** [trivial] will discharge the goal if it's exactly [True] after
 doing normalization and simplification of it. *)
-let trivial : tactic unit = fun () -> TAC?.reflect __trivial
+let trivial () : Tac unit = TAC?.reflect __trivial
 
 assume private val __norm  : list norm_step -> __tac unit
 (** [norm steps] will call the normalizer on the current goal's
@@ -82,18 +82,18 @@ string operations)
 [iota] (reduce match statements over constructors)
 [delta_only] (restrict delta to only unfold this list of fully-qualfied identifiers)
 *)
-let norm steps : tactic unit = fun () -> TAC?.reflect (__norm steps)
+let norm steps : Tac unit = TAC?.reflect (__norm steps)
 
 assume private val __norm_term_env  : env -> list norm_step -> term -> __tac term
 (** [norm_term_env e steps t] will call the normalizer on the term [t]
 using the list of steps [steps], over environment [e]. The list has the same meaning as for [norm]. *)
-let norm_term_env env steps t : tactic term = fun () -> TAC?.reflect (__norm_term_env env steps t)
+let norm_term_env env steps t : Tac term = TAC?.reflect (__norm_term_env env steps t)
 
 assume private val __norm_binder_type  : list norm_step -> binder -> __tac unit
 (** [norm_binder_type steps b] will call the normalizer on the type of the [b]
 binder for the current goal. Notably, this cannot be done via binder_retype and norm,
 because of uvars being resolved to lambda-abstractions. *)
-let norm_binder_type steps b : tactic unit = fun () -> TAC?.reflect (__norm_binder_type steps b)
+let norm_binder_type steps b : Tac unit = TAC?.reflect (__norm_binder_type steps b)
 
 assume private val __intro  : __tac binder
 (** [intro] pushes the first argument of an arrow goal into the
@@ -101,25 +101,25 @@ environment, turning [Gamma |- ?u : x:a -> b] into [Gamma, x:a |- ?u' : b].
 Note that this does not work for logical implications/forall. See
 FStar.Tactics.Logic for that.
 *)
-let intro : tactic binder = fun () -> TAC?.reflect __intro
+let intro () : Tac binder = TAC?.reflect __intro
 
 assume private val __intro_rec  : __tac (binder * binder)
 (** Similar to intros, but allows to build a recursive function.
 Currently broken (c.f. issue #1103)
 *)
-let intro_rec : tactic (binder * binder) = fun () -> TAC?.reflect __intro_rec
+let intro_rec () : Tac (binder * binder) = TAC?.reflect __intro_rec
 
 assume private val __rename_to  : binder -> string -> __tac unit
 (** [rename_to b nm] will rename the binder [b] to [nm] in
 the environment, goal, and witness in a safe manner. The only use of this
 is to make goals and terms more user readable. *)
-let rename_to bv s : tactic unit = fun () -> TAC?.reflect (__rename_to bv s)
+let rename_to bv s : Tac unit = TAC?.reflect (__rename_to bv s)
 
 assume private val __revert  : __tac unit
 (** [revert] pushes out a binder from the environment into the goal type,
 so a behaviour opposite to [intros].
 *)
-let revert : tactic unit = fun () -> TAC?.reflect __revert
+let revert () : Tac unit = TAC?.reflect __revert
 
 assume private val __binder_retype  : binder -> __tac unit
 (** [binder_retype] changes the type of a binder in the context. After calling it
@@ -127,88 +127,88 @@ with a binder of type `t`, the user is presented with a goal of the form `t == ?
 to be filled. The original goal (following that one) has the type of `b` in the
 context replaced by `?u`.
 *)
-let binder_retype (b : binder) : tactic unit = fun () -> TAC?.reflect (__binder_retype b)
+let binder_retype (b : binder) : Tac unit = TAC?.reflect (__binder_retype b)
 
 assume private val __clear_top : __tac unit
 (** [clear_top] will drop the outermost binder from the environment.
 Can only be used if the goal does not at all depend on it.
 *)
-let clear_top : tactic unit = fun () -> TAC?.reflect __clear_top
+let clear_top () : Tac unit = TAC?.reflect __clear_top
 
 assume private val __clear : binder -> __tac unit
 (** [clear] will drop the given binder from the context, is
 nothing depends on it.
 *)
-let clear (b : binder) : tactic unit = fun () -> TAC?.reflect (__clear b)
+let clear (b : binder) : Tac unit = TAC?.reflect (__clear b)
 
 assume private val __rewrite : binder -> __tac unit
 (** If [b] is a binder of type [v == r], [rewrite b] will rewrite
 the variable [v] for [r] everywhere in the current goal type and witness/
 *)
-let rewrite (b:binder) : tactic unit = fun () -> TAC?.reflect (__rewrite b)
+let rewrite (b:binder) : Tac unit = TAC?.reflect (__rewrite b)
 
 assume private val __smt     : __tac unit
 (** [smt] will mark the current goal for being solved through the SMT.
 This does not immediately run the SMT:  it is a marker.
 This tactic never fails, and a goal marked for SMT cannot be brought back. *)
-let smt : tactic unit = fun () -> TAC?.reflect __smt
+let smt () : Tac unit = TAC?.reflect __smt
 
 assume private val __divide: int -> __tac 'a -> __tac 'b -> __tac ('a * 'b)
 (** [divide n t1 t2] will split the current set of goals into the [n]
 first ones, and the rest. It then runs [t1] on the first set, and [t2]
 on the second, returning both results (and concatenating remaining goals). *)
-let divide (n:int) (f:tactic 'a) (g:tactic 'b): tactic ('a * 'b) = fun () -> TAC?.reflect (__divide n (reify_tactic f) (reify_tactic g))
+let divide (n:int) (f:unit -> Tac 'a) (g:unit -> Tac 'b): Tac ('a * 'b) =
+    TAC?.reflect (__divide n (reify (f ())) (reify (g ())))
 
 (* could be implemented using divide *)
 assume private val __seq : __tac unit -> __tac unit -> __tac unit
 (** Runs tactic [t1] on the current goal, and then tactic [t2] on *each*
 subgoal produced by [t1]. Each invocation of [t2] runs on a proofstate
 with a single goal (they're "focused"). *)
-let seq (f:tactic unit) (g:tactic unit) : tactic unit = fun () ->
-  TAC?.reflect (__seq (reify_tactic f) (reify_tactic g))
+let seq (f:unit -> Tac unit) (g:unit -> Tac unit) : Tac unit =
+  TAC?.reflect (__seq (reify (f ())) (reify (g ())))
 
 assume private val __t_exact : bool -> bool -> term -> __tac unit
-let t_exact hard guard (t:tactic term) : tactic unit =
-    fun () -> let tt = t () in TAC?.reflect (__t_exact hard guard tt)
+let t_exact hard guard (t:term) : Tac unit = TAC?.reflect (__t_exact hard guard t)
 
 assume private val __apply : term -> __tac unit
 (** [apply f] will attempt to produce a solution to the goal by an application
 of [f] to any amount of arguments (which need to be solved as further goals).
 The amount of arguments introduced is the least such that [f a_i] unifies
 with the goal's type. *)
-let apply (t:tactic term) : tactic unit = fun () -> let tt = t () in TAC?.reflect (__apply tt)
+let apply (t:term) : Tac unit = TAC?.reflect (__apply t)
 
 assume private val __apply_raw : term -> __tac unit
 (** [apply_raw f] is like [apply], but will ask for all arguments regardless
 of whether they appear free in further goals. *)
-let apply_raw (t:tactic term) : tactic unit = fun () -> let tt = t () in TAC?.reflect (__apply_raw tt)
+let apply_raw (t:term) : Tac unit = TAC?.reflect (__apply_raw t)
 
 assume private val __apply_lemma : term -> __tac unit
 (** [apply_lemma l] will solve a goal of type [squash phi] when [l] is a Lemma
 ensuring [phi]. The arguments to [l] and its requires clause are introduced as new goals.
 As a small optimization, [unit] arguments are discharged by the engine. *)
 // TODO: do the unit thing too for [apply].
-let apply_lemma (t:tactic term) : tactic unit = fun () -> let tt = t () in TAC?.reflect (__apply_lemma tt)
+let apply_lemma (t:term) : Tac unit = TAC?.reflect (__apply_lemma t)
 
 assume private val __print : string -> __tac unit
 (** [print str] has no effect on the proofstate, but will have the side effect
 of printing [str] on the compiler's standard output. *)
-let print (msg:string) : tactic unit = fun () -> TAC?.reflect (__print msg)
+let print (msg:string) : Tac unit = TAC?.reflect (__print msg)
 
 assume private val __dump : string -> __tac unit
 (** Similar to [print], but will dump a text representation of the proofstate
 along with the message. *)
-let dump (msg:string) : tactic unit = fun () -> TAC?.reflect (__dump msg)
+let dump (msg:string) : Tac unit = TAC?.reflect (__dump msg)
 
 assume private val __dump1 : string -> __tac unit
 (** Similar to [dump], but only dumping the current goal. *)
-let dump1 (msg:string) : tactic unit = fun () -> TAC?.reflect (__dump1 msg)
+let dump1 (msg:string) : Tac unit = TAC?.reflect (__dump1 msg)
 
 assume private val __trefl : __tac unit
 (** Solves a goal [Gamma |= squash (l == r)] by attempting to unify
 [l] with [r]. This currently only exists because of some universe problems
 when trying to [apply] a reflexivity lemma. *)
-let trefl : tactic unit = fun () -> TAC?.reflect __trefl
+let trefl () : Tac unit = TAC?.reflect __trefl
 
 assume private val __pointwise : direction -> __tac unit -> __tac unit
 (** (TODO: explain bettter) When running [pointwise tau] For every
@@ -218,12 +218,12 @@ the engine will rewrite [t'] for [?u] in the original goal type. This
 is done for every subterm, bottom-up. This allows to recurse over an
 unknown goal type. By inspecting the goal, the [tau] can then decide
 what to do (to not do anything, use [trefl]). *)
-let pointwise (tau : tactic unit) : tactic unit = fun () -> TAC?.reflect (__pointwise BottomUp (reify_tactic tau))
-let pointwise' (tau : tactic unit) : tactic unit = fun () -> TAC?.reflect (__pointwise TopDown (reify_tactic tau))
+let pointwise  (tau : unit -> Tac unit) : Tac unit = TAC?.reflect (__pointwise BottomUp (reify (tau ())))
+let pointwise' (tau : unit -> Tac unit) : Tac unit = TAC?.reflect (__pointwise TopDown  (reify (tau ())))
 
 assume private val __later : __tac unit
 (** Push the current goal to the back. *)
-let later : tactic unit = fun () -> TAC?.reflect __later
+let later () : Tac unit = TAC?.reflect __later
 
 assume private val __dup : __tac unit
 (** Given the current goal [Gamma |- w : t],
@@ -233,15 +233,15 @@ assume private val __dup : __tac unit
 a goal's witness in any way needed, by choosing
 some [?u] (possibly with exact) and then solving the other goal.
 *)
-let dup : tactic unit = fun () -> TAC?.reflect __dup
+let dup () : Tac unit = TAC?.reflect __dup
 
 assume private val __flip : __tac unit
 (** Flip the order of the first two goals. *)
-let flip : tactic unit = fun () -> TAC?.reflect __flip
+let flip () : Tac unit = TAC?.reflect __flip
 
 assume private val __qed : __tac unit
 (** Succeed if there are no more goals left, and fail otherwise. *)
-let qed : tactic unit = fun () -> TAC?.reflect __qed
+let qed () : Tac unit = TAC?.reflect __qed
 
 // Proof namespace management
 assume private val __prune : string -> __tac unit
@@ -249,11 +249,11 @@ assume private val __prune : string -> __tac unit
 [A.B.C] (and submodules of it) to not be encoded to the SMT, for the current goal.
 The string is a namespace prefix. [prune ""] will prune everything, but note
 that [prune "FStar.S"] will not prune ["FStar.Set"]. *)
-let prune ns : tactic unit = fun () -> TAC?.reflect (__prune ns)
+let prune ns : Tac unit = TAC?.reflect (__prune ns)
 
 assume private val __addns : string -> __tac unit
 (** The opposite operation of [prune]. The latest one takes precedence. *)
-let addns ns : tactic unit = fun () -> TAC?.reflect (__addns ns)
+let addns ns : Tac unit = TAC?.reflect (__addns ns)
 
 assume private val __cases : term -> __tac (term * term)
 (** Given a disjunction [e], destruct it and generate two goals
@@ -261,28 +261,28 @@ for each case. Return value is terms representing proofs for each case.
 The first one is only valid in the first goal, and likewise for
 the second (TODO: change this awful behaviour).
 *)
-let cases t : tactic (term * term) = fun () -> TAC?.reflect (__cases t)
+let cases t : Tac (term * term) = TAC?.reflect (__cases t)
 
 assume private val __set_options : string -> __tac unit
 (** Set command line options for the current goal. Mostly useful to
 change SMT encoding options such as [set_options "--z3rlimit 20"]. *)
-let set_options s : tactic unit = fun () -> TAC?.reflect (__set_options s)
+let set_options s : Tac unit = TAC?.reflect (__set_options s)
 
 assume private val __uvar_env : env -> option typ -> __tac term
 (** Creates a new, unconstrained unification variable in environment
 [env]. The type of the uvar can optionally be provided in [o]. If not
 provided, a second uvar is created for the type. *)
-let uvar_env (e : env) (o : option typ) : tactic term = fun () -> TAC?.reflect (__uvar_env e o)
+let uvar_env (e : env) (o : option typ) : Tac term = TAC?.reflect (__uvar_env e o)
 
 assume private val __unify : term -> term -> __tac bool
 (** Call the unifier on two terms. The return value is whether
 unification was possible. When the tactics returns true, the terms may
 have been instantited by unification. When false, there is no effect. *)
-let unify (t1 t2 : term) : tactic bool = fun () -> TAC?.reflect(__unify t1 t2)
+let unify (t1 t2 : term) : Tac bool = TAC?.reflect(__unify t1 t2)
 
 assume private val __launch_process : string -> string -> string -> __tac string
 (** Launches an external process [prog] with arguments [args] and input
 [input] and returns the output. For security reasons, this can only be
 performed when the `--unsafe_tactic_exec` options was provided for the
 current F* invocation. The tactic will fail if this is not so. *)
-let launch_process (prog args input : string) : tactic string = fun () -> TAC?.reflect (__launch_process prog args input)
+let launch_process (prog args input : string) : Tac string = TAC?.reflect (__launch_process prog args input)
