ulib/FStar.Tactics.Simplifier.fst
@@ -16,11 +16,11 @@ val lem_iff_trans : #a:Type -> #b:Type -> #c:Type -> squash (a <==> b) -> squash
                                                             -> Lemma (a <==> c)
 let lem_iff_trans #a #b #c _ _ = ()
 
-let tiff : tactic unit =
-    apply_lemma (fun () -> `lem_iff_refl)
+let tiff () : Tac unit =
+    apply_lemma (`lem_iff_refl)
 
-let step : tactic unit =
-    apply_lemma (fun () -> `lem_iff_trans)
+let step () : Tac unit =
+    apply_lemma (`lem_iff_trans)
 
 val lem_true_and_p : #p:Type -> Lemma ((True /\ p) <==> p)
 let lem_true_and_p #p = ()
@@ -153,127 +153,126 @@ let is_false t =
            end
     end
 
-val inhabit : tactic unit
-let inhabit =
-    t <-- cur_goal;
+val inhabit : unit -> Tac unit
+let inhabit () =
+    let t = cur_goal () in
     match inspect t with
     | Tv_FVar fv ->
         let qn = inspect_fv fv in
-             if qn = int_lid then exact (fun () -> `42)
-        else if qn = bool_lid then exact (fun () -> `true)
-        else if qn = unit_lid then exact (fun () -> `())
+             if qn = int_lid  then exact (`42)
+        else if qn = bool_lid then exact (`true)
+        else if qn = unit_lid then exact (`())
         else fail ""
     | _ -> fail ""
 
 val simplify_point : unit -> Tac unit
 val recurse : unit -> Tac unit
 
-let rec simplify_point = fun () -> (
-    (* dump "1 ALIVE";; *)
-    recurse;;
-    norm [];;
-    g <-- cur_goal;
+let rec simplify_point () =
+    (* dump "1 ALIVE"; *)
+    recurse ();
+    norm [];
+    let g = cur_goal () in
     let f = term_as_formula g in
-    (* print ("1 g = " ^ term_to_string g);; *)
-    (* print ("1 f = " ^ formula_to_string f);; *)
+    (* print ("1 g = " ^ term_to_string g); *)
+    (* print ("1 f = " ^ formula_to_string f); *)
     match f with
     | Iff l r ->
         begin match term_as_formula' l with
         | And p q ->
-                 if is_true p then apply_lemma (fun () -> `lem_true_and_p)
-            else if is_true q then apply_lemma (fun () -> `lem_p_and_true)
-            else if is_false p then apply_lemma (fun () -> `lem_false_and_p)
-            else if is_false q then apply_lemma (fun () -> `lem_p_and_false)
-            else tiff
+                 if is_true p  then apply_lemma (`lem_true_and_p)
+            else if is_true q  then apply_lemma (`lem_p_and_true)
+            else if is_false p then apply_lemma (`lem_false_and_p)
+            else if is_false q then apply_lemma (`lem_p_and_false)
+            else tiff ()
 
         | Or p q ->
-                 if is_true p then apply_lemma (fun () -> `lem_true_or_p)
-            else if is_true q then apply_lemma (fun () -> `lem_p_or_true)
-            else if is_false p then apply_lemma (fun () -> `lem_false_or_p)
-            else if is_false q then apply_lemma (fun () -> `lem_p_or_false)
-            else tiff
+                 if is_true p  then apply_lemma (`lem_true_or_p)
+            else if is_true q  then apply_lemma (`lem_p_or_true)
+            else if is_false p then apply_lemma (`lem_false_or_p)
+            else if is_false q then apply_lemma (`lem_p_or_false)
+            else tiff ()
 
         | Implies p q ->
-                 if is_true p then apply_lemma (fun () -> `lem_true_imp_p)
-            else if is_true q then apply_lemma (fun () -> `lem_p_imp_true)
-            else if is_false p then apply_lemma (fun () -> `lem_false_imp_p)
-            else tiff
+                 if is_true p  then apply_lemma (`lem_true_imp_p)
+            else if is_true q  then apply_lemma (`lem_p_imp_true)
+            else if is_false p then apply_lemma (`lem_false_imp_p)
+            else tiff ()
 
         | Forall b p ->
-                 if is_true p then apply_lemma (fun () -> `lem_fa_true)
-            else if is_false p then or_else (apply_lemma (fun () -> `lem_fa_false);; inhabit) tiff
-            else tiff
+                 if is_true p  then apply_lemma (`lem_fa_true)
+            else if is_false p then or_else (fun () -> apply_lemma (`lem_fa_false); inhabit ()) tiff
+            else tiff ()
 
         | Exists b p ->
-                 if is_false p then apply_lemma (fun () -> `lem_ex_false)
-            else if is_true  p then or_else (apply_lemma (fun () -> `lem_ex_true);; inhabit) tiff
-            else tiff
+                 if is_false p then apply_lemma (`lem_ex_false)
+            else if is_true  p then or_else (fun () -> apply_lemma (`lem_ex_true); inhabit ()) tiff
+            else tiff ()
 
         | Not p ->
-                 if is_true p then apply_lemma (fun () -> `lem_neg_true)
-            else if is_false p then apply_lemma (fun () -> `lem_neg_false)
-            else tiff
+                 if is_true p  then apply_lemma (`lem_neg_true)
+            else if is_false p then apply_lemma (`lem_neg_false)
+            else tiff ()
 
         | Iff p q ->
             // After applying the lemma, we might still have more simpl to do,
             // so add an intermediate step.
-            step;;
-                 if is_true p then apply_lemma (fun () -> `lem_true_iff_p)
-            else if is_true q then apply_lemma (fun () -> `lem_p_iff_true)
-            else if is_false p then apply_lemma (fun () -> `lem_false_iff_p)
-            else if is_false q then apply_lemma (fun () -> `lem_p_iff_false)
-            else tiff;;
-            simplify_point
+            step ();
+                 if is_true p  then apply_lemma (`lem_true_iff_p)
+            else if is_true q  then apply_lemma (`lem_p_iff_true)
+            else if is_false p then apply_lemma (`lem_false_iff_p)
+            else if is_false q then apply_lemma (`lem_p_iff_false)
+            else tiff ();
+            simplify_point ()
 
-        | _ -> tiff
+        | _ -> tiff ()
         end
     | _ -> fail "simplify_point: failed precondition: goal should be `g <==> ?u`"
-) ()
-and recurse : unit -> Tac unit = fun () -> (
-    (* dump "2 ALIVE";; *)
-    step;;
-    norm [];;
-    g <-- cur_goal;
+
+and recurse () : Tac unit =
+    (* dump "2 ALIVE"; *)
+    step ();
+    norm [];
+    let g = cur_goal () in
     let f = term_as_formula g in
-    (* print ("2 g = " ^ term_to_string g);; *)
-    (* print ("2 f = " ^ formula_to_string f);; *)
+    (* print ("2 g = " ^ term_to_string g); *)
+    (* print ("2 f = " ^ formula_to_string f); *)
     match f with
     | Iff l r ->
         begin match term_as_formula' l with
         | And _ _ ->
-            seq (apply_lemma (fun () -> `and_cong)) simplify_point
+            seq (fun () -> apply_lemma (`and_cong)) simplify_point
 
         | Or _ _ ->
-            seq (apply_lemma (fun () -> `or_cong)) simplify_point
+            seq (fun () -> apply_lemma (`or_cong)) simplify_point
 
         | Implies _ _ ->
-            seq (apply_lemma (fun () -> `imp_cong)) simplify_point
+            seq (fun () -> apply_lemma (`imp_cong)) simplify_point
 
         | Forall _ _ ->
-            apply_lemma (fun () -> `fa_cong);;
-            intro;;
-            simplify_point
+            apply_lemma (`fa_cong);
+            let _ = intro () in
+            simplify_point ()
 
         | Exists _ _ ->
-            apply_lemma (fun () -> `ex_cong);;
-            intro;;
-            simplify_point
+            apply_lemma (`ex_cong);
+            let _ = intro () in
+            simplify_point ()
 
         | Not _ ->
-            apply_lemma (fun () -> `neg_cong);;
-            simplify_point
+            apply_lemma (`neg_cong);
+            simplify_point ()
 
         | Iff _ _ ->
-            seq (apply_lemma (fun () -> `iff_cong)) simplify_point
+            seq (fun () -> apply_lemma (`iff_cong)) simplify_point
 
-        | _ -> tiff
+        | _ -> tiff ()
         end
     | _ -> fail "recurse: failed precondition: goal should be `g <==> ?u`"
-) ()
 
 val equiv : #p:Type -> #q:Type -> squash (p <==> q) -> squash q -> Lemma p
 let equiv #p #q _ _ = ()
 
-let simplify : tactic unit =
-    apply_lemma (fun () -> `equiv);;
-    simplify_point
+let simplify () : Tac unit =
+    apply_lemma (`equiv);
+    simplify_point ()
