examples/tactics/Cut.fst
@@ -10,9 +10,9 @@ assume val p2 : psi -> squash phi
 
 let _ =
     assert_by_tactic phi
-        (psi' <-- quote psi;
-         tcut psi';;
-         flip;;
-         exact (quote p1);; // TODO: kinda pointless example
-         apply (quote p2);;
-         exact (quote p1))
+        (let psi' = quote psi in
+         tcut psi';
+         flip ();
+         exact (`p1); // TODO: kinda pointless example
+         apply (`p2);
+         exact (`p1))
