examples/tactics/NatPos.fst
@@ -2,4 +2,4 @@ module NatPos
 
 open FStar.Tactics
 
-let n : nat = synth_by_tactic (exact (quote 1))
+let n : nat = synth_by_tactic (fun () -> exact (quote 1))
