examples/tactics/Pruning.fst
@@ -59,17 +59,18 @@ let f (x:int) = assert (x + 1 == 1 + x)
 
 // This one should be sent in a pruned context
 let _ = assert_by_tactic (rev [1;2] == [2;1])
-                         (prune "";;
-                          addns "FStar.List";;
-                          addns "Prims")
+                         (fun () -> prune "";
+                                    addns "FStar.List";
+                                    addns "Prims")
 
 // First one should go to the SMT, also in pruned context
 let _ = assert_by_tactic (rev [1;2] == [2;1] /\ 1 == 1)
-                         (prune "";;
-                          FStar.Tactics.split;;
-                          (* rev [1;2] == [2;1] *)
-                              addns "FStar.List";;
-                              addns "Prims";;
-                              smt;;
-                          (* 1 == 1 *)
-                              smt)
+                         (fun () ->
+                            prune "";
+                            FStar.Tactics.split ();
+                            (* rev [1;2] == [2;1] *)
+                                addns "FStar.List";
+                                addns "Prims";
+                                smt ();
+                            (* 1 == 1 *)
+                                smt ())
