examples/tactics/Synthesis.fst
@@ -2,48 +2,50 @@ module Synthesis
 
 open FStar.Tactics
 
-let a : unit = synth_by_tactic (exact (quote ()))
+let a : unit = synth_by_tactic (fun () -> exact (`()))
 
 let _ = assert (a == ())
 
-let rec fib (n : int) : tactic unit =
+let rec fib (n : int) : Tac unit =
     if n < 2
     then
-        exact (quote 1)
+        exact (`1)
     else (
-        apply (quote op_Addition);;
-        iseq [fib (n - 1); fib (n - 2)]
+        apply (`op_Addition);
+        iseq [ (fun () -> fib (n - 1)) ;
+               (fun () -> fib (n - 2)) ]
     )
 
-let f8 : int = synth_by_tactic (fib 8)
+let f8 : int = synth_by_tactic (fun () -> fib 8)
 let _ = assert (f8 == 34) // equal after normalization
 
-let rec fib_norm (n : int) : tactic unit =
+let rec fib_norm (n : int) : Tac unit =
     if n < 2
     then
-        exact (quote 1)
+        exact (`1)
     else (
-        dup;;
-        apply (quote op_Addition);;
-        iseq [fib_norm (n - 1); fib_norm (n - 2)];;
-        norm [primops];;
-        trefl
+        dup ();
+        apply (`op_Addition);
+        iseq [ (fun () -> fib_norm (n - 1)) ;
+               (fun () -> fib_norm (n - 2)) ];
+        norm [primops];
+        trefl ()
     )
 
-let fn8 : int = synth_by_tactic (fib_norm 8)
+let fn8 : int = synth_by_tactic (fun () -> fib_norm 8)
 let _ = assert (fn8 == 34) // syntactically equal
 
 #set-options "--use_two_phase_tc false"  //AR: need to check
 let iszero (x : int) : int =
-    synth_by_tactic (
-        x <-- quote x;
-        t_int <-- quote int;
+    synth_by_tactic (fun () ->
+        let x = quote x in
+        let t_int = quote int in
         let _f = fresh_binder t_int in
         let t = Tv_Match x
                     [(Pat_Constant (C_Int 0), pack (Tv_Const (C_Int 1)));
                      (Pat_Wild _f, pack (Tv_Const (C_Int 0)))] in
-        exact_guard (return (pack t));;
-        smt)
+        exact_guard (pack t);
+        smt ())
 
 let _ = assert (iszero 0 = 1)
 let _ = assert (iszero 1 = 0)
